@@ -1,11 +1,12 @@
 module
 public import Roolean.SmtLib2.Parser
+public import Roolean.SmtLib2.Proof
 
 public class Interpret (α : Type) (ε: outParam Type) where
   new: α
   declareConst: α → String8 → SmtSort → (Except ε α)
   assert : α → SmtTerm → α
-  checkSat : α → IO (Except ε Unit)
+  checkSat : α → SmtProof → IO (Except ε Unit)
 
 public inductive EExecutor (ε : Type)
   | UnsupportedLogic (logic: String8)
@@ -13,7 +14,7 @@ public inductive EExecutor (ε : Type)
 deriving Repr
 
 
-public def execute (α: Type) {ε: Type} [Interpret α ε] (commands: Array SmtCommand): IO ((Except (EExecutor ε)) Unit) := do
+public def execute (α: Type) {ε: Type} [Interpret α ε] (commands: Array SmtCommand) (proof: SmtProof): IO ((Except (EExecutor ε)) Unit) := do
   let mut interpretation: α := Interpret.new
 
   for command in commands do
@@ -34,7 +35,7 @@ public def execute (α: Type) {ε: Type} [Interpret α ε] (commands: Array SmtC
         interpretation := Interpret.assert interpretation term
 
       | .CheckSat =>
-        let result ← Interpret.checkSat interpretation
+        let result ← Interpret.checkSat interpretation proof
         match result with
           | Except.ok () => pure ()
           | Except.error err => return Except.error (EExecutor.Interpretation err)
